format-version: 1.2
date: 30:01:2017 10:44
saved-by: pgaudet
auto-generated-by: OBO-Edit 2.3.1
subsetdef: Terms for voltage-gated sodium channels ""
default-namespace: ICEPO

[Term]
id: ICEPO:0000001
name: conductance
namespace: Electrophysiological parameters
def: "The degree to which electric current carried by the ions flows through a channel symbolized by G and expressed in siemens (S)." [NP:VH]
subset: Terms for voltage-gated sodium channels
xref: http://opal.msu.montana.edu/cftr/ion_channel_glossary.htm
xref: http:www2.montana.edu/cftr/ion_channel_glossary.htm
created_by: vhinard
creation_date: 2015-02-26T10:23:24Z

[Term]
id: ICEPO:0000002
name: ion selectivity
namespace: Electrophysiological parameters
def: "The degree to which a channel allows different ions to pass while excluding others. It is characterized by determining the permeability ratio from the reversal potential (zero net current) under bionic conditions." [NP:VH]
subset: Terms for voltage-gated sodium channels
synonym: "conductive-state ion selectivity" EXACT []
synonym: "ion permeability" RELATED []
xref: PMID:21518830 "Ion selectivity in channels and transporters."
created_by: vhinard
creation_date: 2015-02-26T10:32:40Z

[Term]
id: ICEPO:0000003
name: sodium ion selectivity
namespace: Electrophysiological parameters
def: "The degree to which a channel allows sodium ions to pass while excluding others." [NP:VH]
subset: Terms for voltage-gated sodium channels
xref: PMID:21518830 "Ion selectivity in channels and transporters."
is_a: ICEPO:0000002 ! ion selectivity
created_by: vhinard
creation_date: 2015-02-26T10:34:49Z

[Term]
id: ICEPO:0000004
name: activation
namespace: Electrophysiological parameters
def: "The transition from the closed to the open state of the channel. It relates the opening of a channel due to the presence of a gating signal, allowing the transfer of ions through the pore." [NP:VH]
subset: Terms for voltage-gated sodium channels
synonym: "activation gating" RELATED []
synonym: "opening" EXACT []
xref: https://wiki.brown.edu/confluence/download/attachments/13802/Ion+Channels+Glossary.pdf
xref: ISBN:0878933212 "Ion channels of excitable membranes - Bertil Hille - 2001"
created_by: vhinard
creation_date: 2015-02-26T10:35:53Z

[Term]
id: ICEPO:0000005
name: time dependence of activation
namespace: Electrophysiological parameters
def: "The rate of activation of the channel." [NP:VH]
subset: Terms for voltage-gated sodium channels
synonym: "activation kinetics" EXACT []
relationship: part_of ICEPO:0000004 ! activation
created_by: vhinard
creation_date: 2015-02-26T10:37:40Z

[Term]
id: ICEPO:0000006
name: voltage dependence of activation
namespace: Electrophysiological parameters
def: "The opening of the channel in relation to the electrochemical driving force (voltage)." [NP:VH]
comment: Measured by a steady-state activation curve (V1/2).
subset: Terms for voltage-gated sodium channels
synonym: "voltage dependence of steady-state activation" EXACT []
xref: ISBN:0878933212 "Ion channels of excitable membranes - Bertil Hille - 2001"
is_a: ICEPO:0000040 ! stimulus dependence of activation
created_by: vhinard
creation_date: 2015-02-26T10:38:54Z

[Term]
id: ICEPO:0000007
name: inactivation
namespace: Electrophysiological parameters
def: "The transition from open to inactivated state of the channel. It relates the closing of the channel in the continued presence of the gating signal. The channel is then in a refractory period. No ion can pass through the pore and it is unresponsive to stimulus." [NP:VH]
subset: Terms for voltage-gated sodium channels
synonym: "inactivated state" RELATED []
synonym: "inactivation gating" RELATED []
synonym: "open-state inactivation" RELATED []
xref: https://wiki.brown.edu/confluence/download/attachments/13802/Ion+Channels+Glossary.pdf
xref: ISBN:0878933212 "Ion channels of excitable membranes - Bertil Hille - 2001"
created_by: vhinard
creation_date: 2015-02-26T10:39:35Z

[Term]
id: ICEPO:0000008
name: fast inactivation
namespace: Electrophysiological parameters
def: "The fast phase of inactivation from the open-state of the channel." [NP:VH]
subset: Terms for voltage-gated sodium channels
synonym: "fast open-state inactivation" RELATED []
xref: ISBN:0878933212 "Ion channels of excitable membranes - Bertil Hille - 2001"
relationship: part_of ICEPO:0000007 ! inactivation
created_by: vhinard
creation_date: 2015-02-26T10:40:53Z

[Term]
id: ICEPO:0000009
name: entry into fast inactivated state
namespace: Electrophysiological parameters
def: "The transition rate to reach the fast inactivated state." [NP:VH]
comment: Measured either by decay phase or peak-to-baseline analysis during whole cell recording.
subset: Terms for voltage-gated sodium channels
synonym: " entry into fast inactivation" RELATED []
synonym: "decay phase" RELATED []
synonym: "fast-gated kinetics" RELATED []
xref: ISBN:0878933212 "Ion channels of excitable membranes - Bertil Hille - 2001"
relationship: part_of ICEPO:0000016 ! time dependence of fast inactivation
created_by: vhinard
creation_date: 2015-02-26T10:41:24Z

[Term]
id: ICEPO:0000010
name: voltage dependence of fast inactivation
namespace: Electrophysiological parameters
def: "Fast inactivation of the channel in relation to the electrochemical driving force (voltage)." [NP:VH]
comment: Measured by a steady-state fast inactivation curve (V1/2).
subset: Terms for voltage-gated sodium channels
synonym: "voltage dependence of fast open-state inactivation" RELATED []
synonym: "voltage-dependent channel availability" RELATED []
xref: ISBN:0878933212 "Ion channels of excitable membranes - Bertil Hille - 2001"
is_a: ICEPO:0000037 ! stimulus dependence of fast inactivation
created_by: vhinard
creation_date: 2015-02-26T10:41:56Z

[Term]
id: ICEPO:0000011
name: slow inactivation
namespace: Electrophysiological parameters
def: "The slow phase of inactivation from the open-state of the channel." [NP:VH]
subset: Terms for voltage-gated sodium channels
synonym: "slow open-state inactivation" RELATED []
xref: ISBN:0878933212 "Ion channels of excitable membranes - Bertil Hille - 2001"
relationship: part_of ICEPO:0000007 ! inactivation
created_by: vhinard
creation_date: 2015-02-26T10:43:26Z

[Term]
id: ICEPO:0000012
name: entry into slow inactivated state
namespace: Electrophysiological parameters
def: "The transition rate to reach the slow inactivated state." [NP:VH]
subset: Terms for voltage-gated sodium channels
synonym: "entry into slow open-state inactivation" RELATED []
synonym: "onset of slow inactivation" RELATED []
xref: ISBN:0878933212 "Ion channels of excitable membranes - Bertil Hille - 2001"
relationship: part_of ICEPO:0000018 ! time dependence of slow inactivation
created_by: vhinard
creation_date: 2015-02-26T10:44:06Z

[Term]
id: ICEPO:0000013
name: voltage dependence of slow inactivation
namespace: Electrophysiological parameters
def: "Slow inactivation of the channel in relation to the electrochemical driving force (voltage)." [NP:VH]
comment: Measured by a steady-state slow inactivation curve (V1/2).
subset: Terms for voltage-gated sodium channels
synonym: "voltage dependence of slow open-state inactivation" RELATED []
xref: ISBN:0878933212 "Ion channels of excitable membranes - Bertil Hille - 2001"
is_a: ICEPO:0000041 ! stimulus dependence of slow inactivation
created_by: vhinard
creation_date: 2015-02-26T10:44:37Z

[Term]
id: ICEPO:0000014
name: recovery
namespace: Electrophysiological parameters
def: "The transition from the inactivated to the closed state in which the channel is non-conducting." [NP:VH]
subset: Terms for voltage-gated sodium channels
synonym: "closing" EXACT []
xref: ISBN:0878933212 "Ion channels of excitable membranes - Bertil Hille - 2001"
created_by: vhinard
creation_date: 2015-02-26T10:45:09Z

[Term]
id: ICEPO:0000015
name: recovery from fast inactivation
namespace: Electrophysiological parameters
def: "The transition from fast inactivation to closed state." [NP:VH]
subset: Terms for voltage-gated sodium channels
synonym: "recovery from fast open-state inactivation" RELATED []
synonym: "repriming" EXACT []
xref: ISBN:0878933212 "Ion channels of excitable membranes - Bertil Hille - 2001"
relationship: part_of ICEPO:0000014 ! recovery
created_by: vhinard
creation_date: 2015-02-26T10:45:54Z

[Term]
id: ICEPO:0000016
name: time dependence of fast inactivation
namespace: Electrophysiological parameters
def: "The rate of fast inactivation of the channel." [NP:VH]
subset: Terms for voltage-gated sodium channels
is_a: ICEPO:0000008 ! fast inactivation
created_by: vhinard
creation_date: 2015-02-26T10:46:26Z

[Term]
id: ICEPO:0000017
name: recovery from slow inactivation
namespace: Electrophysiological parameters
def: "The transition from slow inactivation to closed state." [NP:VH]
subset: Terms for voltage-gated sodium channels
synonym: "recovery from slow open-state inactivation" RELATED []
xref: ISBN:0878933212 "Ion channels of excitable membranes - Bertil Hille - 2001"
relationship: part_of ICEPO:0000014 ! recovery
created_by: vhinard
creation_date: 2015-02-26T10:46:58Z

[Term]
id: ICEPO:0000018
name: time dependence of slow inactivation
namespace: Electrophysiological parameters
def: "The rate of slow inactivation of the channel." [NP:VH]
subset: Terms for voltage-gated sodium channels
relationship: part_of ICEPO:0000011 ! slow inactivation
created_by: vhinard
creation_date: 2015-02-26T10:47:53Z

[Term]
id: ICEPO:0000019
name: deactivation
namespace: Electrophysiological parameters
def: "The transition from the open to the closed state of the channel." [NP:VH]
subset: Terms for voltage-gated sodium channels
synonym: "Open-state deactivation" RELATED []
xref: ISBN:0878933212 "Ion channels of excitable membranes - Bertil Hille - 2001"
created_by: vhinard
creation_date: 2015-02-26T10:49:27Z

[Term]
id: ICEPO:0000020
name: calcium ion selectivity
namespace: Electrophysiological parameters
def: "The degree to which a channel allows calcium ions to pass while excluding others." [NP:VH]
xref: PMID:21518830 "Ion selectivity in channels and transporters."
is_a: ICEPO:0000002 ! ion selectivity
created_by: vhinard
creation_date: 2015-11-30T12:48:15Z

[Term]
id: ICEPO:0000021
name: reopening
namespace: Electrophysiological parameters
def: "The transition from the inactivated to the open state of the channel." [NP:VH]
subset: Terms for voltage-gated sodium channels
synonym: "resurgent current" RELATED []
xref: ISBN:0878933212 "Ion channels of excitable membranes - Bertil Hille - 2001"
created_by: vhinard
creation_date: 2015-02-26T10:50:43Z

[Term]
id: ICEPO:0000022
name: chloride ion selectivity
namespace: Electrophysiological parameters
def: "The degree to which a channel allows chloride ions to pass while excluding others." [NP:VH]
xref: PMID:21518830 "Ion selectivity in channels and transporters."
is_a: ICEPO:0000002 ! ion selectivity
created_by: vhinard
creation_date: 2015-11-30T12:48:35Z

[Term]
id: ICEPO:0000023
name: potassium ion selectivity
namespace: Electrophysiological parameters
def: "The degree to which a channel allows potassium ions to pass while excluding others." [NP:VH]
xref: PMID:21518830 "Ion selectivity in channels and transporters."
is_a: ICEPO:0000002 ! ion selectivity
created_by: vhinard
creation_date: 2015-02-26T03:18:22Z

[Term]
id: ICEPO:0000024
name: voltage sensitivity of activation
namespace: Electrophysiological parameters
def: "The capacity of the channel to respond to voltage changes during activation." [NP:VH]
comment: Measured by the slope of a steady-state activation curve (k, slope factor).
subset: Terms for voltage-gated sodium channels
xref: ISBN:0878933212 "Ion channels of excitable membranes - Bertil Hille - 2001"
relationship: part_of ICEPO:0000006 ! voltage dependence of activation
created_by: pgaudet
creation_date: 2015-03-26T02:16:09Z

[Term]
id: ICEPO:0000025
name: stimulus dependence of recovery from fast inactivation
namespace: Electrophysiological parameters
def: "The recovery from fast inactivation of the channel in relation to the stimulus." [NP:VH]
subset: Terms for voltage-gated sodium channels
relationship: part_of ICEPO:0000015 ! recovery from fast inactivation
created_by: vhinard
creation_date: 2015-10-22T10:40:17Z

[Term]
id: ICEPO:0000026
name: voltage sensitivity of fast inactivation
namespace: Electrophysiological parameters
def: "The capacity of the channel to respond to voltage changes during fast inactivation." [NP:VH]
comment: Measured by the slope of a steady-state fast inactivation curve (k, slope factor).
subset: Terms for voltage-gated sodium channels
xref: ISBN:0878933212 "Ion channels of excitable membranes - Bertil Hille - 2001"
relationship: part_of ICEPO:0000010 ! voltage dependence of fast inactivation
created_by: pgaudet
creation_date: 2015-03-26T02:21:37Z

[Term]
id: ICEPO:0000027
name: voltage sensitivity of slow inactivation
namespace: Electrophysiological parameters
def: "The capacity of the channel to respond to voltage changes during slow inactivation." [NP:VH]
comment: Measured by the slope of a steady-state slow inactivation curve (k, slope factor).
subset: Terms for voltage-gated sodium channels
xref: ISBN:0878933212 "Ion channels of excitable membranes - Bertil Hille - 2001"
relationship: part_of ICEPO:0000013 ! voltage dependence of slow inactivation
created_by: pgaudet
creation_date: 2015-03-26T02:21:56Z

[Term]
id: ICEPO:0000028
name: macroscopic conductance
namespace: Electrophysiological parameters
def: "The degree to which electric current carried by the ions flows through a population of channels in a macropatch expressed as a current in Ampere (A)." [NP:VH]
subset: Terms for voltage-gated sodium channels
synonym: "current density (pA/pF)" RELATED []
synonym: "normalized conductance (G/Gmax)" RELATED []
synonym: "normalized current (I/Imax)" RELATED []
xref: ISBN:0878933212 "Ion channels of excitable membranes - Bertil Hille - 2001"
is_a: ICEPO:0000001 ! conductance
created_by: pgaudet
creation_date: 2015-03-26T02:22:49Z

[Term]
id: ICEPO:0000029
name: single channel conductance
namespace: Electrophysiological parameters
def: "The degree to which electric current carried by the ions flows through a single channel in a membrane patch expressed in Siemens (S)." [NP:VH]
subset: Terms for voltage-gated sodium channels
synonym: "current amplitude" RELATED []
xref: ISBN:0878933212 "Ion channels of excitable membranes - Bertil Hille - 2001"
is_a: ICEPO:0000001 ! conductance
created_by: pgaudet
creation_date: 2015-03-26T02:23:04Z

[Term]
id: ICEPO:0000030
name: entry into activated state
namespace: Electrophysiological parameters
def: "The transition rate to reach the activated state." [NP:VH]
comment: Measured either by time to peak current analysis during whole cell recording or by latency to first opening and open probability analysis during single channel recording.
subset: Terms for voltage-gated sodium channels
synonym: "<new synonym>" RELATED []
synonym: "latency to first opening" RELATED []
synonym: "open probability" RELATED []
synonym: "time to peak current" RELATED []
xref: ISBN:0878933212 "Ion channels of excitable membranes - Bertil Hille - 2001"
relationship: part_of ICEPO:0000005 ! time dependence of activation
created_by: vhinard
creation_date: 2015-04-30T08:59:09Z

[Term]
id: ICEPO:0000031
name: development of activation
namespace: Electrophysiological parameters
def: "The time spent into the open state." [NP:VH]
comment: Measured by the mean open time during single channel recording.
subset: Terms for voltage-gated sodium channels
synonym: "open duration" RELATED []
synonym: "open time" RELATED []
xref: ISBN:0878933212 "Ion channels of excitable membranes - Bertil Hille - 2001"
relationship: part_of ICEPO:0000005 ! time dependence of activation
created_by: vhinard
creation_date: 2015-04-30T09:05:42Z

[Term]
id: ICEPO:0000032
name: development of fast inactivation
namespace: Electrophysiological parameters
def: "The time spent into fast inactivated state." [NP:VH]
subset: Terms for voltage-gated sodium channels
xref: ISBN:0878933212 "Ion channels of excitable membranes - Bertil Hille - 2001"
relationship: part_of ICEPO:0000016 ! time dependence of fast inactivation
created_by: vhinard
creation_date: 2015-04-30T09:07:51Z

[Term]
id: ICEPO:0000033
name: development of slow inactivation
namespace: Electrophysiological parameters
def: "The time spent into slow inactivated state." [NP:VH]
subset: Terms for voltage-gated sodium channels
xref: ISBN:0878933212 "Ion channels of excitable membranes - Bertil Hille - 2001"
relationship: part_of ICEPO:0000018 ! time dependence of slow inactivation
created_by: vhinard
creation_date: 2015-04-30T09:11:24Z

[Term]
id: ICEPO:0000034
name: closed-state inactivation
namespace: Electrophysiological parameters
def: "The transition from the closed to the inactivated state, more precisely from a pre-open closed-state directly to the inactivated state." [NP:VH]
subset: Terms for voltage-gated sodium channels
synonym: "closed-state fast inactivation" EXACT []
xref: ISBN:0878933212 "Ion channels of excitable membranes - Bertil Hille - 2001"
created_by: vhinard
creation_date: 2015-05-06T08:37:01Z

[Term]
id: ICEPO:0000035
name: voltage dependence of recovery from fast inactivation
namespace: Electrophysiological parameters
def: "Recovery from fast inactivation of the channel in relation to the electrochemical driving force (voltage)." [NP:VH]
subset: Terms for voltage-gated sodium channels
xref: ISBN:0878933212 "Ion channels of excitable membranes - Bertil Hille - 2001"
is_a: ICEPO:0000025 ! stimulus dependence of recovery from fast inactivation
created_by: vhinard
creation_date: 2015-07-28T10:07:23Z

[Term]
id: ICEPO:0000036
name: voltage dependence of recovery from slow inactivation
namespace: Electrophysiological parameters
def: "Recovery from slow inactivation of the channel in relation to the electrochemical driving force (voltage)." [NP:VH]
subset: Terms for voltage-gated sodium channels
xref: ISBN:0878933212 "Ion channels of excitable membranes - Bertil Hille - 2001"
is_a: ICEPO:0000042 ! stimulus dependence of recovery from slow inactivation
created_by: vhinard
creation_date: 2015-07-28T10:09:48Z

[Term]
id: ICEPO:0000037
name: stimulus dependence of fast inactivation
namespace: Electrophysiological parameters
def: "The fast inactivation of the channel in relation to the stimulus." [NP:VH]
subset: Terms for voltage-gated sodium channels
is_a: ICEPO:0000008 ! fast inactivation
created_by: vhinard
creation_date: 2015-10-16T15:37:17Z

[Term]
id: ICEPO:0000038
name: voltage sensitivity of recovery from fast inactivation
namespace: Electrophysiological parameters
def: "The capacity of the channel to respond to voltage changes during recovery from fast inactivation." [NP:VH]
subset: Terms for voltage-gated sodium channels
xref: ISBN:0878933212 "Ion channels of excitable membranes - Bertil Hille - 2001"
relationship: part_of ICEPO:0000035 ! voltage dependence of recovery from fast inactivation
created_by: vhinard
creation_date: 2015-07-28T10:11:11Z

[Term]
id: ICEPO:0000039
name: voltage sensitivity of recovery from slow inactivation
namespace: Electrophysiological parameters
def: "The capacity of the channel to respond to voltage changes during recovery from slow inactivation." [NP:VH]
subset: Terms for voltage-gated sodium channels
xref: ISBN:0878933212 "Ion channels of excitable membranes - Bertil Hille - 2001"
relationship: part_of ICEPO:0000036 ! voltage dependence of recovery from slow inactivation
created_by: vhinard
creation_date: 2015-07-28T10:12:41Z

[Term]
id: ICEPO:0000040
name: stimulus dependence of activation
namespace: Electrophysiological parameters
def: "The opening of the channel in relation to the stimulus." [NP:VH]
comment: The stimulus can be the voltage, ligand, temperature, light or cell deformation.
subset: Terms for voltage-gated sodium channels
relationship: part_of ICEPO:0000004 ! activation
created_by: vhinard
creation_date: 2015-10-16T14:41:11Z

[Term]
id: ICEPO:0000041
name: stimulus dependence of slow inactivation
namespace: Electrophysiological parameters
def: "The slow inactivation of the channel in relation to the stimulus." [NP:VH]
subset: Terms for voltage-gated sodium channels
relationship: part_of ICEPO:0000011 ! slow inactivation
created_by: vhinard
creation_date: 2015-10-22T09:59:10Z

[Term]
id: ICEPO:0000042
name: stimulus dependence of recovery from slow inactivation
namespace: Electrophysiological parameters
def: "The recovery from slow inactivation of the channel in relation to the stimulus." [NP:VH]
subset: Terms for voltage-gated sodium channels
relationship: part_of ICEPO:0000017 ! recovery from slow inactivation
created_by: vhinard
creation_date: 2015-10-22T10:45:24Z

[Term]
id: ICEPO:0000043
name: time dependence of recovery from fast inactivation
namespace: Electrophysiological parameters
def: "The rate of recovery from fast inactivation of the channel." [NP:VH]
relationship: part_of ICEPO:0000015 ! recovery from fast inactivation
created_by: vhinard
creation_date: 2015-10-22T10:49:29Z

[Term]
id: ICEPO:0000044
name: entry into the closed state from the fast inactivation
namespace: Electrophysiological parameters
def: "The transition rate to reach the closed state from the fast inactivation." [NP:VH]
comment: Measured by the closed probability analysis during single channel recording.
synonym: "closed probability" RELATED []
xref: ISBN:0878933212 "Ion channels of excitable membranes - Bertil Hille - 2001"
is_a: ICEPO:0000043 ! time dependence of recovery from fast inactivation
created_by: vhinard
creation_date: 2015-10-22T10:50:18Z

[Term]
id: ICEPO:0000045
name: development of closed state from fast inactivation
namespace: Electrophysiological parameters
def: "The time spent into the closed state from fast inactivation." [NP:VH]
comment: Measured by the mean closed time during single channel recording.
synonym: "closed time" RELATED []
xref: ISBN:0878933212 "Ion channels of excitable membranes - Bertil Hille - 2001"
is_a: ICEPO:0000043 ! time dependence of recovery from fast inactivation
created_by: vhinard
creation_date: 2015-10-22T10:52:22Z

[Term]
id: ICEPO:0000046
name: time dependence of recovery from slow inactivation
namespace: Electrophysiological parameters
def: "The rate of recovery from slow inactivation of the channel." [NP:VH]
relationship: part_of ICEPO:0000017 ! recovery from slow inactivation
created_by: vhinard
creation_date: 2015-10-22T11:01:08Z

[Term]
id: ICEPO:0000047
name: development of closed state from slow inactivation
namespace: Electrophysiological parameters
def: "The time spent into the closed state  from slow inactivation." [NP:VH]
xref: ISBN:0878933212 "Ion channels of excitable membranes - Bertil Hille - 2001"
is_a: ICEPO:0000046 ! time dependence of recovery from slow inactivation
created_by: vhinard
creation_date: 2015-10-22T11:02:15Z

[Term]
id: ICEPO:0000048
name: entry into the closed state from the slow inactivation
namespace: Electrophysiological parameters
def: "The transition rate to reach the closed state from the slow inactivation." [NP:VH]
xref: ISBN:0878933212 "Ion channels of excitable membranes - Bertil Hille - 2001"
is_a: ICEPO:0000046 ! time dependence of recovery from slow inactivation
created_by: vhinard
creation_date: 2015-10-22T11:02:38Z

[Typedef]
id: part_of
name: part of
namespace: Electrophysiological parameters
subset: Terms for voltage-gated sodium channels
is_transitive: true

